Some more progress

Picinae_calling.v
@@ -33,97 +33,6 @@ Open Scope bool.
 Open Scope list.
 Open Scope N.
 
-Definition set A := list A.
-Definition eqb {A} {eq: EqDec A} (a b: A): bool :=
-  if a == b then true else false.
-Arguments eqb {A} {eq} (a b): simpl never.
-Definition set_elems {A} (s: set A): list A := s.
-Definition set_exists {A} {e: EqDec A} (s: set A) (a: A): bool :=
-  existsb (eqb a) s.
-Definition set_nil {A}: set A := nil.
-Definition set_add {A} {e: EqDec A} (s: set A) (a: A): set A :=
-  if set_exists s a then s else a :: s.
-Definition set_ap {A} {e: EqDec A} (s1 s2: set A): set A :=
-  filter (fun a => negb (set_exists s2 a)) s1 ++ s2.
-
-Theorem eqb_refl: forall A {e: EqDec A} (a: A), eqb a a = true.
-Proof.
-  intros. unfold eqb.
-  destruct (a == a); [reflexivity|].
-  destruct n. reflexivity.
-Qed.
-
-Theorem eqb_eq: forall A {e: EqDec A} (a a': A), a = a' <-> eqb a a' = true.
-Proof.
-  intros. unfold eqb.
-  destruct (a == a'). split; intro; [reflexivity|assumption].
-  split; intro; [destruct n; assumption|discriminate].
-Qed.
-
-Theorem eqb_neq: forall A {e: EqDec A} (a a': A), a <> a' <-> eqb a a' = false.
-Proof.
-  intros. unfold eqb.
-  destruct (a == a'). split; intro; [destruct H; assumption|discriminate].
-  split; intro; [reflexivity|assumption].
-Qed.
-
-Theorem set_ex_add_frame: forall A {e: EqDec A} (s: set A) (a a': A)
-  (NE: a' <> a), set_exists (set_add s a) a' = set_exists s a'.
-Proof.
-  intros. unfold set_add, set_exists.
-  destruct (existsb _ s) eqn: EX; [reflexivity|]. simpl.
-  rewrite (proj1 (eqb_neq _ _ _) NE). reflexivity.
-Qed.
-
-Theorem set_ex_add_this: forall A {e: EqDec A} (s: set A) (a: A),
-  set_exists (set_add s a) a = true.
-Proof.
-  intros. unfold set_add, set_exists.
-  destruct (existsb _ s) eqn: EX; [assumption|]. simpl. rewrite eqb_refl.
-  reflexivity.
-Qed.
-
-Theorem set_ex_ap_orb: forall A {e: EqDec A} (s1 s2: set A) (a: A),
-  set_exists (set_ap s1 s2) a = set_exists s1 a || set_exists s2 a.
-Proof.
-  intros. unfold set_ap, set_exists.
-
-  (* Found in s2 *)
-  destruct (existsb _ s2) eqn: EX2. rewrite existsb_app, EX2, orb_true_r,
-  Bool.orb_true_r. reflexivity.
-
-  (* Not in s2... *)
-  rewrite existsb_app, EX2, orb_false_r, orb_false_r.
-
-  (* ... but in s1 *)
-  destruct (existsb _ s1) eqn: EX1. apply existsb_exists. eexists.
-  apply existsb_exists in EX1. destruct EX1 as [a' [In Eq]].
-  apply eqb_eq in Eq. subst. split; [|apply eqb_refl]. apply filter_In.
-  split; [assumption|]. rewrite EX2. reflexivity.
-
-  (* ... or not in either *)
-  destruct (existsb _ (filter _ _)) eqn: EX12; [|reflexivity].
-  apply existsb_exists in EX12. destruct EX12 as [a' [In Eq]].
-  apply eqb_eq in Eq. subst. apply filter_In in In. destruct In as [InS1 _].
-  symmetry. rewrite <- EX1. apply existsb_exists. eexists.
-  split; [eassumption|apply eqb_refl].
-Qed.
-
-Corollary set_ex_ap_or: forall A {e: EqDec A} (s1 s2: set A) (a: A),
-  set_exists s1 a = true \/ set_exists s2 a = true ->
-  set_exists (set_ap s1 s2) a = true.
-Proof.
-  intros. rewrite set_ex_ap_orb. apply orb_true_intro. assumption.
-Qed.
-
-Corollary set_ex_ap_l: forall A {e: EqDec A} (s1 s2: set A) (a: A)
-  (EX1: set_exists s1 a = true), set_exists (set_ap s1 s2) a = true.
-Proof. intros. apply set_ex_ap_or. left. assumption. Qed.
-
-Corollary set_ex_ap_r: forall A {e: EqDec A} (s1 s2: set A) (a: A)
-  (EX2: set_exists s2 a = true), set_exists (set_ap s1 s2) a = true.
-Proof. intros. apply set_ex_ap_or. right. assumption. Qed.
-
 (* partial functions *)
 Definition pfunc (A B:Type) := A -> option B.
 Bind Scope pfunc_scope with pfunc.
@@ -133,192 +42,124 @@ Notation "x ⇀ y" := (pfunc x y) (at level 99, y at level 200, right associativ
 (* the empty function (bottom) *)
 Notation "⊥" := (fun _ => None).
 
-(* composition of partial functions *)
-Definition pcompose {A:Type} (f g : A ⇀ A) (x : A) :=
-  match g x with None => None | Some y => f y end.
-Notation "f ○ g" := (pcompose f g) (at level 40, g at next level, left associativity) : pfunc_scope.
+Inductive simple_exp :=
+  | Number (n: N) (w: bitwidth)
+  | VarOff (v: var) (off: N) (w: bitwidth)
+  | Complex.
 
-Definition pupdate {A B} {e: EqDec A} (s: A ⇀ B) (key: A) (val: B): pfunc A B :=
-  fun key' => if key' == key then Some val else s key'.
+Definition store_delta := var -> simple_exp.
 
-Definition premove {A B} {e: EqDec A} (s: A ⇀ B) (key: A): pfunc A B :=
-  fun key' => if key' == key then None else s key'.
-
-Theorem pupdate_frame: forall A B {e: EqDec A} (s: pfunc A B) (key key': A) val
-  (NE: key' ≠ key), (pupdate s key val) key' = s key'.
-Proof.
-  intros. unfold pupdate. destruct (key' == key); [|reflexivity]. destruct NE.
-  assumption.
-Qed.
-
-Theorem premove_frame: forall A B {e: EqDec A} (s: pfunc A B) (key key': A)
-  (NE: key' ≠ key), (premove s key) key' = s key'.
-Proof.
-  intros. unfold premove. destruct (key' == key); [|reflexivity]. destruct NE.
-  assumption.
-Qed.
-
-Theorem pupdate_this: forall A B {e: EqDec A} (s: pfunc A B) (key: A) val,
-  (pupdate s key val) key = Some val.
-Proof.
-  intros. unfold pupdate. destruct (iseq_refl key). rewrite H. reflexivity.
-Qed.
-
-Theorem premove_this: forall A B {e: EqDec A} (s: pfunc A B) (key: A),
-  (premove s key) key = None.
-Proof.
-  intros. unfold premove. destruct (iseq_refl key). rewrite H. reflexivity.
-Qed.
-
-Fixpoint get_jumps (s: stmt): option (set addr) :=
-  match s with
-  | Nop => Some set_nil
-  | Move _ _ => Some set_nil
-  | Jmp e =>
-      match e with
-      | Word loc _ => Some (set_add set_nil loc)
-      | _ => None
-      end
-  | Exn _ => Some set_nil
-  | Seq s1 s2 | If _ s1 s2 =>
-      match (get_jumps s1, get_jumps s2) with
-      | (_, None) => None
-      | (None, _) => None
-      | (Some j1, Some j2) => Some (set_ap j1 j2)
-      end
-  | Rep _ s => get_jumps s
+Definition sexp_width (e: simple_exp) :=
+  match e with
+  | Number _ w => Some w
+  | VarOff _ _ w => Some w
+  | Complex => None
   end.
 
-Lemma jump_rep_total: forall e q h s s' x a
-  (XS: exec_stmt h s (Rep e q) s' x) (EX: x = Some a),
-  exists s0 s0', exec_stmt h s0 q s0' x.
+Inductive hastyp_simple_exp (c: typctx): simple_exp -> typ -> Prop :=
+  | TSE_Num (n: N) (w: bitwidth) (LT: n < 2 ^ w):
+      hastyp_simple_exp c (Number n w) (NumT w)
+  | TSE_VarOff (v: var) (w: bitwidth) (off: N) (CV: c v = Some (NumT w))
+      (LT: off < 2 ^ w): hastyp_simple_exp c (VarOff v off w) (NumT w).
+
+Lemma hastyp_simple_exp_num:
+  forall c e t (TSE: hastyp_simple_exp c e t), exists w, t = NumT w.
 Proof.
-  intros. inversion XS; subst; clear XS; simpl in *.
-  rewrite N2Nat.inj_iter in XS0. remember (N.to_nat n) as nn.
-  clear e w E n Heqnn. revert q h s s' a XS0.
-  induction nn; intros. inversion XS0. inversion XS0; subst; clear XS0.
-  - eexists. eexists. eassumption.
-  - eapply IHnn. eassumption.
+  intros. inversion TSE; eexists; reflexivity.
 Qed.
 
-Theorem get_jumps_complete: forall q h s0 s1 x a' jmps
-  (XS: exec_stmt h s0 q s1 x) (EX: x = Some (Exit a'))
-  (JMPS: Some jmps = get_jumps q), set_exists jmps a' = true.
+Lemma sexp_width_type_correct: forall c e w (TSE: hastyp_simple_exp c e (NumT w)),
+  sexp_width e = Some w.
 Proof.
-  induction q; intros; inversion XS; subst; simpl in *; try discriminate.
-  - (* Jmp *) inversion E; subst; simpl in *; clear E; try discriminate.
-    inversion H2. subst. inversion JMPS. apply set_ex_add_this.
-  - (* Seq, exit in q1 *) destruct (get_jumps q1) eqn: J1;
-    destruct (get_jumps q2) eqn: J2; try discriminate. inversion JMPS. subst.
-    clear JMPS. apply set_ex_ap_l. eapply IHq1. eassumption. assumption. reflexivity.
-  - (* Seq, exit in q2 *) destruct (get_jumps q1) eqn: J1;
-    destruct (get_jumps q2) eqn: J2; try discriminate. inversion JMPS. subst.
-    clear JMPS. apply set_ex_ap_r. eapply IHq2. eassumption. reflexivity. reflexivity.
-  - (* If *) destruct (get_jumps q1) eqn: J1; destruct (get_jumps q2) eqn: J2;
-    try discriminate. inversion JMPS. subst. clear JMPS. apply set_ex_ap_or.
-    destruct c; [right; eapply IHq2|left; eapply IHq1];
-        try solve [eassumption|reflexivity].
-  - (* Evil rep *) destruct (jump_rep_total _ _ _ _ _ _ _ XS eq_refl) as
-    [s2 [s3 SInner]]. eapply IHq; solve [reflexivity|eassumption].
+  intros. inversion TSE; reflexivity.
 Qed.
 
-Parameter sp_reg: var
-(* Definition sp_reg := R_ESP*).
-
-Parameter reg_bitwidth: bitwidth
-(* Definition reg_bitwidth: bitwidth := 32. *).
-
-Inductive stack_exp :=
-  | Imm (w: bitwidth) (n: N)
-  | SPOff (off: N)
-  | UnkVal.
-
-Definition sexp_width (e: stack_exp) :=
+Fixpoint simplify_exp (c0: typctx) (δ: store_delta) e :=
   match e with
-  | Imm w _ => Some w
-  | SPOff _ => Some reg_bitwidth
-  | UnkVal => None
-  end.
-
-Fixpoint classify_exp0 st e :=
-  match e with
-  | Var v => st v
-  | Word n w => Imm w n
-  | Load _ _ _ _ => UnkVal
-  | Store _ _ _ _ _ => UnkVal
+  | Var v => δ v
+  | Word n w => Number n w
+  | Load _ _ _ _ => Complex
+  | Store _ _ _ _ _ => Complex
   | BinOp op e1 e2 =>
-      let of_oper sp_off n (is_inverted: bool) :=
-        match op with
-        | OP_PLUS => if is_inverted then
-            SPOff ((n + sp_off) mod 2 ^ reg_bitwidth)
-          else
-            SPOff ((sp_off + n) mod 2 ^ reg_bitwidth)
-        | OP_MINUS => if is_inverted then UnkVal else
-            SPOff ((sp_off + 2 ^ reg_bitwidth - n) mod 2 ^ reg_bitwidth)
-        | _ => UnkVal
+      let of_oper v offset n (is_inverted: bool) :=
+        match c0 v with
+        | Some (NumT w) =>
+            match op with
+            | OP_PLUS => if is_inverted then
+                VarOff v ((n + offset) mod 2 ^ w) w
+              else
+                VarOff v ((offset + n) mod 2 ^ w) w
+            | OP_MINUS => if is_inverted then Complex else
+                VarOff v ((offset + 2 ^ w - n) mod 2 ^ w) w
+            | _ => Complex
+            end
+        | None | Some (MemT _) => Complex
         end in
-      match classify_exp0 st e1, classify_exp0 st e2 with
-      | UnkVal, _ | _, UnkVal | SPOff _, SPOff _ => UnkVal
-      | Imm w1 n1, Imm w2 n2 =>
+      match simplify_exp c0 δ e1, simplify_exp c0 δ e2 with
+      | Complex, _ | _, Complex | VarOff _ _ _, VarOff _ _ _ => Complex
+      | Number n1 w1, Number n2 w2 =>
           if w1 == w2 then
             match eval_binop op w1 n1 n2 with
-            | VaN n w' => Imm w' n
-            | VaM _ _ => UnkVal
+            | VaN n w' => Number n w'
+            | VaM _ _ => Complex
             end
-          else UnkVal
-      | SPOff off1, Imm w2 n2 =>
-          if w2 == reg_bitwidth then of_oper off1 n2 false
-          else UnkVal
-      | Imm w1 n1, SPOff off2 =>
-          if w1 == reg_bitwidth then of_oper off2 n1 true
-          else UnkVal
+          else Complex
+      | VarOff v1 off1 w1, Number n2 w2 =>
+          if w1 == w2 then of_oper v1 off1 n2 false
+          else Complex
+      | Number n1 w1, VarOff v2 off2 w2 =>
+          if w1 == w2 then of_oper v2 off2 n1 true
+          else Complex
       end
-  | UnOp _ _ => UnkVal
+  | UnOp _ _ => Complex
   | Cast typ w' e =>
-      let se := classify_exp0 st e in
+      let se := simplify_exp c0 δ e in
       match sexp_width se with
       | Some w =>
           match se with
-          | Imm _ n => Imm w' (cast typ w w' n)
-          | SPOff _ =>
+          | Number n _ => Number (cast typ w w' n) w'
+          | VarOff _ _ _ =>
               match typ with
               | CAST_LOW | CAST_HIGH => (* narrowing *)
-                  if w <=? w' then se else UnkVal
+                  if w <=? w' then se else Complex
               | CAST_UNSIGNED | CAST_SIGNED => (* widening *)
-                  if w' <=? w then se else UnkVal
+                  if w' <=? w then se else Complex
               end
-          | UnkVal => UnkVal
+          | Complex => Complex
           end
-      | None => UnkVal
+      | None => Complex
       end
   | Let v e e_in =>
-      if sp_reg == v then UnkVal
-      else classify_exp0 (fun v' =>
-        if v' == v then classify_exp0 st e else st v') e_in
-  | Unknown _ => UnkVal
-  | Ite _ _ _ => UnkVal
-  | Extract _ _ _ => UnkVal
-  | Concat _ _ => UnkVal
+      simplify_exp c0 (update δ v (simplify_exp c0 δ e)) e_in
+  | Unknown _ => Complex
+  | Ite _ _ _ => Complex
+  | Extract _ _ _ => Complex
+  | Concat _ _ => Complex
   end.
 
-Definition classify_exp (e: exp): stack_exp :=
-   classify_exp0 (fun v' => if sp_reg == v' then SPOff 0 else UnkVal) e.
+Inductive eval_stack_exp (s: store): simple_exp -> value -> Prop :=
+  | ESE_Number n w: eval_stack_exp s (Number n w) (VaN n w)
+  | ESE_VarOff v n off w (SV: s v = VaN n w): eval_stack_exp s
+      (VarOff v off w) (VaN ((n + off) mod 2 ^ w) w).
 
-Inductive eval_stack_exp (s: store): stack_exp -> value -> Prop :=
-  | ESE_Imm w n: eval_stack_exp s (Imm w n) (VaN n w)
-  | ESE_SPOff sp off (S_SP: s sp_reg = VaN sp reg_bitwidth):
-      eval_stack_exp s (SPOff off) (VaN ((sp + off) mod 2 ^ reg_bitwidth) reg_bitwidth).
+Lemma eval_stack_exp_num: forall s se v (ESE: eval_stack_exp s se v),
+  exists n w, v = VaN n w.
+Proof.
+  intros. inversion ESE; subst; clear ESE; eexists; eexists; reflexivity.
+Qed.
 
-Definition stack_equiv (s: store) (st: var → stack_exp) :=
-  forall var val, eval_stack_exp s (st var) val -> s var = val.
+Definition has_delta (s s': store) (δ: store_delta) :=
+  forall v val (ESE: eval_stack_exp s (δ v) val), s' v = val.
 
-Definition stack_models (c: typctx) (st: var → stack_exp) :=
-  forall v b b' (CV: c v = Some (NumT b)) (SEW: Some b' = sexp_width (st v)),
-  b = b'.
+Definition delta_safety (c0: typctx) (δ: store_delta) :=
+  forall v0 v off w (EQ_V: (δ v) = VarOff v0 off w), c0 v0 = Some (NumT w).
 
+Definition delta_models (c: typctx) (δ: store_delta) :=
+  forall v t (CV: c v = Some t), hastyp_simple_exp c (δ v) t.
+
+(*
 Theorem stack_equiv_imp_models: forall c s st
-  (C_SP: c sp_reg = Some (NumT reg_bitwidth)) (MDL: models c s)
-  (SEQ: stack_equiv s st), stack_models c st.
+  (MDL: models c s) (SEQ: stack_equiv s st), stack_models c st.
 Proof.
   unfold stack_models. intros.
   specialize (MDL _ _ CV) as MDL_V. inversion MDL_V. subst. clear MDL_V.
@@ -326,13 +167,13 @@ Proof.
   destruct (st v) eqn: ST; inversion SEW; subst; clear SEW.
   - (* Imm *) erewrite SEQ in H0; [|rewrite ST; constructor]. inversion H0.
     reflexivity.
-  - (* SPOff *) erewrite SEQ in H0; [|rewrite ST; constructor;
+  - (* VarOff *) erewrite SEQ in H0; [|rewrite ST; constructor;
     symmetry; eassumption]. inversion H0. reflexivity.
 Qed.
 
-Theorem preservation_classify_exp0: forall e w w' c st
+Theorem preservation_simplify_exp0: forall e w w' c st
   (ETyp: hastyp_exp c e (NumT w)) (SMDL: stack_models c st)
-  (ESBits: Some w' = sexp_width (classify_exp0 st e))
+  (ESBits: Some w' = sexp_width (simplify_exp0 st e))
   (C_SP: c sp_reg = Some (NumT reg_bitwidth)), w = w'.
 Proof.
   intros.
@@ -343,8 +184,8 @@ Proof.
   - (* Word *) inversion ESBits. inversion ETyp. reflexivity.
   - (* Binop *) inversion ETyp. subst. clear ETyp. simpl in ESBits.
     specialize (IHe1 st). specialize (IHe2 st).
-    destruct (classify_exp0 _ e1) eqn: C1; try discriminate;
-    destruct (classify_exp0 _ e2) eqn: C2; try discriminate;
+    destruct (simplify_exp0 _ e1) eqn: C1; try discriminate;
+    destruct (simplify_exp0 _ e2) eqn: C2; try discriminate;
     destruct (_ == _) eqn: EQB; try discriminate;
     destruct b; try solve
       [ discriminate
@@ -353,12 +194,12 @@ Proof.
   - (* Cast *) inversion ETyp. subst. clear ETyp. simpl in ESBits.
     specialize (IHe st). destruct (sexp_width _) eqn: SEW; try discriminate.
     replace b with w1; [| eapply IHe; solve [eassumption|reflexivity]].
-    destruct (classify_exp0 _ _) eqn: C1; try discriminate.
+    destruct (simplify_exp0 _ _) eqn: C1; try discriminate.
 
     (* Imm *)
     inversion ESBits. reflexivity.
 
-    (* SPOff *)
+    (* VarOff *)
     inversion SEW. subst. clear SEW. assert (w1 = reg_bitwidth);
       [eapply IHe; solve [eassumption|reflexivity]|subst].
     destruct c; destruct (_ <=? _) eqn: LEB; try discriminate;
@@ -377,51 +218,99 @@ Proof.
       - subst. rewrite update_frame in CV by assumption. eapply SMDL; eassumption.
     }
 Qed.
+*)
 
-Theorem classify_exp0_red: forall e h s vs ve c t st
-  (ETyp: hastyp_exp c e t) (MDL: models c s) (SEQ: stack_equiv s st)
-  (EE: eval_exp h s e ve) (ESE: eval_stack_exp s (classify_exp0 st e) vs)
-  (SP_Reg: c sp_reg = Some (NumT reg_bitwidth)), ve = vs.
+Theorem preservation_simplify_exp: forall e t c δ
+  (ETyp: hastyp_exp c e t) (DMDL: delta_models c δ),
+  hastyp_simple_exp c (simplify_exp c δ e) t.
+Proof.
+Admitted.
+
+Corollary preservation_bitwidth_simplify_exp: forall e c δ w
+  (TE: hastyp_exp c e (NumT w)) (DMDL: delta_models c δ),
+  sexp_width (simplify_exp c δ e) = Some w.
+Proof.
+  intros. eapply sexp_width_type_correct. eapply preservation_simplify_exp;
+  eassumption.
+Qed.
+
+Theorem simplify_exp_correct: forall e h s0 s δ vs ve c t
+  (ETyp: hastyp_exp c e t) (MDL0: models c s0) (MDL: models c s)
+  (DS: delta_safety c δ) (DMDL: delta_models c δ) (HD: has_delta s0 s δ)
+  (EE: eval_exp h s e ve) (ESE: eval_stack_exp s0 (simplify_exp c δ e) vs), ve = vs.
 Proof.
   intros.
+
+  (* Specify vs *)
+  apply eval_stack_exp_num in ESE as VS. destruct VS as [n' [w' VS]]. subst.
+
+  (*
   assert (SMDL: stack_models c st). eapply stack_equiv_imp_models; eassumption.
   (* assert SP < 2 ^ reg_bitwidth *)
   specialize (MDL sp_reg _ SP_Reg) as MDL_SP. inversion MDL_SP. subst.
   symmetry in H0. clear MDL_SP.
-  revert c s st n LT H0 vs ve t SMDL MDL ETyp SP_Reg SEQ EE ESE.
+   *)
+  revert c s δ n' w' ve t MDL0 MDL DMDL DS HD ETyp EE ESE.
   induction e; intros; try solve [inversion ESE].
-  - (* Var *) inversion EE. subst. apply SEQ. assumption.
+  - (* Var *) inversion EE. subst. eapply HD. eassumption.
   - (* Word *) inversion EE. inversion ESE. subst. reflexivity.
   - (* BinOp *) inversion EE. inversion ETyp. subst. clear EE ETyp.
-    assert (2 ^ reg_bitwidth <> 0). destruct reg_bitwidth; discriminate.
-    simpl in ESE. destruct (classify_exp0 _ e1) eqn: C1; try solve [inversion ESE];
-    destruct (classify_exp0 _ e2) eqn: C2; try solve [inversion ESE];
-    destruct (w1 == _) eqn: EQW; try solve [inversion ESE];
-    (* Push the inductive hypothesis *)
-    (eassert (Equiv1: VaN n1 w = VaN _ _);[eapply IHe1;
-      solve [eassumption|rewrite C1; econstructor; eassumption] |] );
-    (eassert (Equiv2: VaN n2 w = VaN _ _);[eapply IHe2;
-      solve [eassumption|rewrite C2; econstructor; eassumption] |] );
-    inversion Equiv1; inversion Equiv2; subst; clear IHe1 IHe2 Equiv1 Equiv2.
-    + (* imm OP imm *) destruct (eval_binop _ _ n0 n3) eqn: Ev; [|inversion ESE].
-      inversion ESE. subst. clear ESE. rewrite <- Ev. reflexivity.
-    + (* imm OP SP *) destruct b; inversion ESE; subst; clear ESE. simpl.
-      specialize (preservation_eval_exp MDL T1 E1) as TV. inversion TV. subst.
-      rewrite H0 in S_SP. inversion S_SP. subst.
-      erewrite <- (N.mod_small n0) at 1; [|eassumption].
-      erewrite <- (N.mod_small sp) at -1; [|eassumption].
+
+    (* Clean up some of the bitwidth variables, to ensure w = w0 *)
+    eassert (TV1: hastyp_val _ _). eapply (preservation_eval_exp MDL T1);
+      eassumption.
+    eassert (TV2: hastyp_val _ _). eapply (preservation_eval_exp MDL T2);
+      eassumption.
+    eassert (TSE1: hastyp_simple_exp _ (simplify_exp _ _ e1) _).
+      eapply preservation_simplify_exp; eassumption.
+    eassert (TSE2: hastyp_simple_exp _ (simplify_exp _ _ e2) _).
+      eapply preservation_simplify_exp; eassumption.
+    inversion TV1. inversion TV2. subst. clear TV1 TV2 H5.
+
+    (* This is a common assumption that we will have to make *)
+    assert (2 ^ w0 <> 0). destruct w0; discriminate.
+
+    (* Do a bunch of case destructions *)
+    simpl in ESE. destruct (simplify_exp _ _ e1) eqn: C1; try solve [inversion ESE];
+    destruct (simplify_exp _ _ e2) eqn: C2; try solve [inversion ESE];
+    destruct (w == _) eqn: EQW; try solve [inversion ESE];
+    try destruct (c v) eqn: CV; try solve [inversion ESE];
+    try destruct t; try solve [inversion ESE];
+    inversion TSE1; inversion TSE2; subst;
+    destruct b; simpl in ESE; inversion ESE; subst; clear ESE;
+    try (rewrite CV0 in CV; inversion CV; subst; clear CV);
+
+    (* Push indutive hypothesis*)
+    (eassert (Equiv1: VaN n1 _ = VaN _ _); [
+      eapply IHe1; solve [eassumption|rewrite C1; econstructor; eassumption]
+    |]); inversion Equiv1; subst; clear Equiv1;
+    (eassert (Equiv2: VaN n2 _ = VaN _ _); [
+      eapply IHe2; solve [eassumption|rewrite C2; econstructor; eassumption]
+    |]); inversion Equiv2; subst; clear Equiv2;
+
+    (* Trivial cases for imm OP imm *)
+    try reflexivity;
+
+    (* Next we need to extract condition for register to be smaller than 2 ^ w' *)
+    (eassert (TV: hastyp_val _ _); [eapply MDL0; eassumption|
+    inversion TV; rewrite SV in H1; inversion H1; subst; clear TV H1; simpl]).
+
+      (* imm + var *)
+      erewrite <- (N.mod_small n) at 1 by eassumption.
+      erewrite <- (N.mod_small n0) at -1; [|eassumption].
       repeat rewrite <- N.add_mod by assumption. f_equal. f_equal.
-      rewrite N.add_assoc, (N.add_comm n0), <- N.add_assoc. reflexivity.
-    + (* SP OP imm *) destruct b; inversion ESE; subst; clear ESE;
-      specialize (preservation_eval_exp MDL T2 E2) as TV; inversion TV; subst;
-      rewrite H0 in S_SP; inversion S_SP; subst.
-      (* OP_PLUS *) simpl. erewrite <- (N.mod_small n0) at 1; [|eassumption].
-      erewrite <- (N.mod_small sp) at -1; [|eassumption].
+      rewrite N.add_assoc, N.add_assoc. f_equal. apply N.add_comm.
+
+      (* var + imm *)
+      erewrite <- (N.mod_small n) at 1 by eassumption.
+      erewrite <- (N.mod_small n0) at -1; [|eassumption].
       repeat rewrite <- N.add_mod by assumption. f_equal. f_equal.
       rewrite N.add_assoc. reflexivity.
-      (* OP_MINUS *) unfold eval_binop, towidth. rewrite N.add_comm. f_equal.
+
+      (* var - imm *)
+      rewrite N.add_comm. f_equal.
       apply N.lt_le_incl in LT0. rewrite <- N.add_sub_assoc, <- N.add_sub_assoc,
-        N.add_mod, N.mod_mod, <- N.add_mod, (N.add_mod sp), N.mod_mod,
+        N.add_mod, N.mod_mod, <- N.add_mod, (N.add_mod n0), N.mod_mod,
       <- N.add_mod, N.add_assoc by assumption. reflexivity.
   - (* Cast *) inversion EE. inversion ETyp. subst.
     specialize (preservation_eval_exp MDL T1 E1) as TV. inversion TV. subst.
@@ -429,21 +318,21 @@ Proof.
     (* sexp_width _ = Some w1 *)
     clear EE ETyp TV. simpl in ESE. destruct (sexp_width _) eqn: EQW;
       try solve [inversion ESE]. symmetry in EQW.
-    assert (w1 = b). eapply preservation_classify_exp0; eassumption. subst.
+    assert (w1 = b). eapply preservation_simplify_exp0; eassumption. subst.
 
     (* Speciailize IH *)
     assert (IHe2: forall ve vs, eval_exp h s e ve ->
-      eval_stack_exp s (classify_exp0 st e) vs -> ve = vs).
+      eval_stack_exp s (simplify_exp0 st e) vs -> ve = vs).
     intros. eapply IHe; eassumption.
 
-    destruct (classify_exp0 _ e) eqn: C'; try solve [inversion ESE].
+    destruct (simplify_exp0 _ e) eqn: C'; try solve [inversion ESE].
 
     (* For Imm *)
     inversion ESE. subst. clear ESE. f_equal. f_equal.
     assert (Equiv1: VaN n0 b = VaN n1 w0). eapply IHe2;
     try solve [eassumption|constructor]. inversion Equiv1. reflexivity.
 
-    (* For SPOff *)
+    (* For VarOff *)
     destruct c; destruct (_ <=? _) eqn: LEB; try solve [inversion ESE];
     apply N.leb_le in LEB; (assert (w = b); [apply N.le_antisymm;
     eassumption|subst]).
@@ -456,8 +345,8 @@ Proof.
     + (* CAST_UNSIGNED *) simpl. eapply IHe2; try eassumption.
   - (* Let *) inversion EE. inversion ETyp. subst. clear EE ETyp.
     simpl in ESE. destruct (sp_reg == v). inversion ESE.
-    eassert (ESE': eval_stack_exp (s[_ := _]) (classify_exp0 _ e2) vs). {
-      destruct (classify_exp0 _ e2) eqn: C2; rewrite C2; inversion ESE; subst.
+    eassert (ESE': eval_stack_exp (s[_ := _]) (simplify_exp0 _ e2) vs). {
+      destruct (simplify_exp0 _ e2) eqn: C2; rewrite C2; inversion ESE; subst.
       - constructor.
       - constructor. rewrite update_frame. assumption. eassumption.
     }
@@ -466,7 +355,7 @@ Proof.
     (* S_SP' *) rewrite update_frame by assumption. assumption.
     (* SMDL' *) unfold stack_models. intros. { destruct (v0 == v).
       - subst. rewrite update_updated in CV. inversion CV.
-        subst. clear CV. eapply preservation_classify_exp0; eassumption.
+        subst. clear CV. eapply preservation_simplify_exp0; eassumption.
       - subst. rewrite update_frame in CV by assumption. eapply SMDL; eassumption.
     }
     (* MDL *) unfold models. intros. { destruct (v0 == v).
@@ -478,7 +367,7 @@ Proof.
     (* SP_REG' *) rewrite update_frame by assumption. assumption.
     (* SEQ' *) unfold stack_equiv. intros v0 val ESE1. { destruct (v0 == v).
       - subst. rewrite update_updated. eapply IHe1; try eassumption.
-        destruct (classify_exp0 _ e1) eqn: C1; inversion ESE1; subst.
+        destruct (simplify_exp0 _ e1) eqn: C1; inversion ESE1; subst.
         + constructor.
         + constructor. rewrite update_frame in S_SP by assumption. assumption.
       - rewrite update_frame by assumption. eapply SEQ.
@@ -488,12 +377,12 @@ Proof.
     }
 Qed.
 
-Theorem classify_exp_red: forall e h s vs ve c t
+Theorem simplify_exp_red: forall e h s vs ve c t
   (ETyp: hastyp_exp c e t) (MDL: models c s)
-  (EE: eval_exp h s e ve) (ESE: eval_stack_exp s (classify_exp e) vs)
+  (EE: eval_exp h s e ve) (ESE: eval_stack_exp s (simplify_exp e) vs)
   (SP_Reg: c sp_reg = Some (NumT reg_bitwidth)), ve = vs.
 Proof.
-  intros. eapply classify_exp0_red; try eassumption.
+  intros. eapply simplify_exp0_red; try eassumption.
   unfold stack_equiv. intros v0 val ESE1.
   destruct (sp_reg == v0); inversion ESE1; subst; clear ESE1.
   rewrite S_SP. f_equal. rewrite N.add_0_r, N.mod_small. reflexivity.
@@ -510,29 +399,29 @@ Definition check_fallthru must_fall (x: option exit) :=
   must_fall = false \/ x = None.
 
 Inductive exec_stack_oper (s: store):
-  (option exit -> Prop) -> stack_oper -> Prop :=
-  | ESO_UpdateSP s' e off v must_fall (ESE: eval_stack_exp s e v)
-      (E_SPOff: e = SPOff off): exec_stack_oper s (s[sp_reg := v])
+  store -> (option exit -> Prop) -> stack_oper -> Prop :=
+  | ESO_UpdateSP e off v must_fall (ESE: eval_stack_exp s e v)
+      (E_VarOff: e = VarOff off): exec_stack_oper s (s[sp_reg := v])
       (check_fallthru must_fall) (SPOper must_fall off)
   | ESO_OtherOper must_fall: exec_stack_oper s s
       (check_fallthru must_fall) (OtherOper must_fall).
 
 (* Classifies a statement by what it does to the stack. *)
-Fixpoint classify_stmt (q: stmt): stack_oper :=
+Fixpoint simplify_stmt (q: stmt): stack_oper :=
   match q with
   | Nop => OtherOper true
   | Move v e =>
       if sp_reg == v then
-        match classify_exp e with
+        match simplify_exp e with
         | Imm _ _ => ErrorOper
-        | SPOff off => SPOper true off
-        | UnkVal => ErrorOper
+        | VarOff off => SPOper true off
+        | Complex => ErrorOper
         end
       else OtherOper true
   | Jmp _ => OtherOper false
   | Exn _ => OtherOper false
   | Seq q1 q2 =>
-      match classify_stmt q1, classify_stmt q2 with
+      match simplify_stmt q1, simplify_stmt q2 with
       | OtherOper true, x | x, OtherOper true => x
       | SPOper true off, OtherOper false => SPOper false off
       | SPOper true off1, SPOper true off2 => SPOper true (off1 + off2)
@@ -540,24 +429,24 @@ Fixpoint classify_stmt (q: stmt): stack_oper :=
       | _, _ => ErrorOper
       end
   | If _ q1 q2 =>
-      match classify_stmt q1, classify_stmt q2 with
+      match simplify_stmt q1, simplify_stmt q2 with
       | OtherOper falls, OtherOper falls2 =>
           OtherOper (falls && falls2)%bool
       | _, _ => ErrorOper
       end
   | Rep _ s =>
-      match classify_stmt s with
+      match simplify_stmt s with
       | OtherOper falls => OtherOper falls
       | _ => ErrorOper
       end
   end.
 
 (*
-Lemma classify_rep_stmt_red: forall q e h s s' x
+Lemma simplify_rep_stmt_red: forall q e h s s' x
   (EX: exec_stmt h s (Rep e q) s' x)
   (IHq : ∀ (s s' : store) (x : option exit) (EX : exec_stmt h s q s' x),
-        exec_stack_oper h s q s' x EX (classify_stmt q)),
-  match classify_stmt q with
+        exec_stack_oper h s q s' x EX (simplify_stmt q)),
+  match simplify_stmt q with
   | SNop => x = None /\ s sp_reg = s' sp_reg
   | SOther => s sp_reg = s' sp_reg
   | _ => True
@@ -568,19 +457,19 @@ Proof.
   remember (N.to_nat n) as nn. clear n Heqnn. move nn at top. move IHq at top.
   repeat match goal with [H: _ |- _] => revert H end.
   induction nn; intros.
-  - (* n = 0 *) inversion XS. subst. clear XS. destruct classify_stmt;
+  - (* n = 0 *) inversion XS. subst. clear XS. destruct simplify_stmt;
     constructor; reflexivity.
   - (* n > 0 *) inversion XS; subst; clear XS.
 
     (* Terminated loop at this step *)
     specialize (IHq _ _ _ XS0).
-    destruct classify_stmt; try solve [constructor]; inversion IHq.
+    destruct simplify_stmt; try solve [constructor]; inversion IHq.
     discriminate. assumption.
 
     (* Continue onwards in the loop *)
     specialize (IHq _ _ _ XS1).
     specialize (IHnn _ _ _ XS0).
-    destruct classify_stmt; try solve [constructor]; inversion IHq.
+    destruct simplify_stmt; try solve [constructor]; inversion IHq.
 
     destruct IHnn. split. assumption.
     all: eapply eq_trans; eassumption.
@@ -589,15 +478,16 @@ Qed.
 Ltac fallthrus :=
   (left + right); reflexivity.
 
-Theorem classify_stmt_red_sp: forall q h s s' s1' x c0 c1 c' Xcond
-  (XS: exec_stmt h s q s' x) (ESO: exec_stack_oper s s1' Xcond (classify_stmt q))
+Theorem simplify_stmt_red_sp: forall q h s s' s1' x c0 c1 c' Xcond
+  (XS: exec_stmt h s q s' x) (ESO: exec_stack_oper s s1' Xcond (simplify_stmt q))
   (STyp: hastyp_stmt c0 c1 q c'), Xcond x /\ s' sp_reg = s1' sp_reg.
 Proof.
   induction q; intros; simpl in *;
   inversion STyp; subst; clear STyp.
   - (* Nop *) inversion XS. inversion ESO. subst. clear XS ESO. split.
-    fallthrus. assumption.
-  - (* Move *) inversion XS. subst. destruct (sp_reg == v);
+    fallthrus. reflexivity.
+  - (* Move *) inversion XS. split. inversion ESO; fallthrus. subst.
+    destruct (sp_reg == v);
     [|constructor; [|reflexivity]; rewrite update_frame; [reflexivity|assumption]].
     (* Destruct on expression. For the error cases, anything happens, so ignore *)
     inversion E; subst; clear E; try constructor;
@@ -618,8 +508,8 @@ Proof.
     econstructor. eassumption. reflexivity. rewrite N.add_comm. reflexivity.
   - (* Jmp *) inversion XS. subst. constructor. reflexivity.
   - (* Exn *) inversion XS. subst. constructor. reflexivity.
-  - (* Seq *) inversion XS; subst; destruct (classify_stmt q1) eqn: C1;
-    destruct (classify_stmt q2) eqn: C2; try constructor; inversion XS; subst;
+  - (* Seq *) inversion XS; subst; destruct (simplify_stmt q1) eqn: C1;
+    destruct (simplify_stmt q2) eqn: C2; try constructor; inversion XS; subst;
     try solve
       [ (* When we execute only the first statement, but it is SNop *)
         specialize (IHq1 _ _ _ _ _ _ _ XS0 TS1); inversion IHq1;
@@ -643,14 +533,14 @@ Proof.
   - (* If *) inversion XS. subst. clear E. clear c' TE SS. destruct c;
     [ specialize (IHq2 _ _ _ _ _ _ _ XS TS2); rename IHq2 into IHq
     | specialize (IHq1 _ _ _ _ _ _ _ XS TS1); rename IHq1 into IHq];
-    destruct (classify_stmt q1) eqn: C1; destruct (classify_stmt q2) eqn: C2;
+    destruct (simplify_stmt q1) eqn: C1; destruct (simplify_stmt q2) eqn: C2;
     inversion IHq; subst; constructor; solve [reflexivity|assumption].
   - (* Rep *) assert (IHq2: ∀ (s s' : store) (x : option exit)
-      (XS : exec_stmt h s q s' x), exec_stack_oper h s q s' x XS (classify_stmt q)).
+      (XS : exec_stmt h s q s' x), exec_stack_oper h s q s' x XS (simplify_stmt q)).
     intros. eapply IHq; eassumption.
-    specialize (classify_rep_stmt_semequiv _ _ _ _ _ _ XS IHq2) as Eq.
+    specialize (simplify_rep_stmt_semequiv _ _ _ _ _ _ XS IHq2) as Eq.
 
-    destruct (classify_stmt) eqn: CS; try constructor.
+    destruct (simplify_stmt) eqn: CS; try constructor.
     destruct Eq. assumption. destruct Eq. assumption.
     assumption.
 Qed.
@@ -658,9 +548,9 @@ Qed.
 Require Import Picinae_i386.
 Require Import strchr_i386.
 Definition null_state: store := fun _ => VaN 0 0.
-Definition classify_stmt_at (p: program) (a: addr): option (N * stack_oper) :=
+Definition simplify_stmt_at (p: program) (a: addr): option (N * stack_oper) :=
   match p null_state a with
-  | Some (sz, q) => Some (sz, classify_stmt q)
+  | Some (sz, q) => Some (sz, simplify_stmt q)
   | None => None
   end.
 
@@ -679,7 +569,7 @@ Compute rev (filter
             | Some _ => true
             | None => false
             end)
-  (map (fun a => (a, classify_stmt_at fstat_i386 a)) (addrs 450))).
+  (map (fun a => (a, simplify_stmt_at fstat_i386 a)) (addrs 450))).
 
 
 Fixpoint push_stack_offsets (p: program) (a: addr): option (set addr, ) :=
